Refactor up to Values.v

src/PlutusIR/Semantics/Dynamic/Values.v
@@ -21,108 +21,13 @@ Inductive value : Term -> Prop :=
       value (Constant u)
   | V_Error : forall T,
       value (Error T)
-  (** Builtins *)
-  | V_Neutral : forall nv,
-      neutral_value 0 nv ->
-      value nv
-  (** If-Then-Else constructs
-
-      NOTE (2021-11-4): Removed separate treatment of if-then-else for the sake of simplicity.
-  *)
-  (* | V_If :
-      value (Builtin IfThenElse)
-  | V_If1 : forall T,
-      value (TyInst (Builtin IfThenElse) T)
-  | V_If2 : forall T cond,
-      value (Apply (TyInst (Builtin IfThenElse) T) cond)
-  | V_If3 : forall T cond t,
-      value (Apply (Apply (TyInst (Builtin IfThenElse) T) cond) t) *)
-
-with neutral_value : nat -> Term -> Prop :=
-  | NV_Builtin : forall n f,
-      (* NOTE (2021-11-4): Removed separate treatment of if-then-else for the sake of simplicity. *)
-      (* f <> IfThenElse -> *)
-      n < arity f ->
-      neutral_value n (Builtin f)
-  | NV_Apply : forall n nv v,
-      value v ->
-      ~ is_error v ->
-      neutral_value (S n) nv ->
-      neutral_value n (Apply nv v)
-  | NV_TyInst : forall n nv T,
-      neutral_value (S n) nv ->
-      neutral_value n (TyInst nv T)
-  .
+.
 
 #[export] Hint Constructors value : core.
-#[export] Hint Constructors neutral_value : core.
 
-Scheme value__ind := Minimality for value Sort Prop
-  with neutral_value__ind := Minimality for neutral_value Sort Prop.
-
-Combined Scheme value__multind from
-  value__ind,
-  neutral_value__ind.
-
-Definition neutral (t : Term) := neutral_value 0 t.
-
-#[export] Hint Unfold neutral : core.
-
-Inductive fully_applied_neutral : nat -> Term -> Prop :=
-  | FA_Builtin : forall n f,
-      (* NOTE (2021-11-4): Removed separate treatment of if-then-else for the sake of simplicity. *)
-      (* f <> IfThenElse -> *)
-      n = arity f ->
-      fully_applied_neutral n (Builtin f)
-  | FA_Apply : forall n nv v,
-      value v ->
-      ~ is_error v ->
-      fully_applied_neutral (S n) nv ->
-      fully_applied_neutral n (Apply nv v)
-  | FA_TyInst : forall n nv T,
-      fully_applied_neutral (S n) nv ->
-      fully_applied_neutral n (TyInst nv T)
-  .
-
-#[export] Hint Constructors fully_applied_neutral : core.
-
-Definition fully_applied (t : Term) := fully_applied_neutral 0 t.
-
-#[export] Hint Unfold fully_applied : core.
+Scheme value__ind := Minimality for value Sort Prop.
 
 Require Import Lia.
-
-Lemma neutral_value__monotone : forall n m nv,
-    neutral_value n nv ->
-    m <= n ->
-    neutral_value m nv.
-Proof with (eauto || (try lia)).
-  intros.
-  generalize dependent m.
-  induction H; intros...
-  - destruct f...
-    all: econstructor...
-  - econstructor...
-    eapply IHneutral_value...
-  - econstructor...
-    eapply IHneutral_value...
-Qed.
-
-Lemma fully_applied_neutral__subsumes__neutral_value : forall m n nv,
-  fully_applied_neutral n nv ->
-  m < n ->
-  neutral_value m nv.
-Proof with (eauto || (try lia)).
-  intros.
-  generalize dependent m.
-  induction H; intros...
-  - subst...
-  - econstructor...
-    eapply IHfully_applied_neutral...
-  - econstructor...
-    eapply IHfully_applied_neutral...
-Qed.
-
 
 Definition is_error_b (t : Term) :=
   match t with
@@ -138,35 +43,16 @@ Proof.
 Qed.
 
 Fixpoint
-  dec_value' (n : nat) (t : Term) {struct t} :=
+  dec_value (t : Term) {struct t} :=
   match t with
     | LamAbs x T t0 => true
     | TyAbs X K t   => true
-    | IWrap F T v   => dec_value' n v && negb (is_error_b v)
+    | IWrap F T v   => dec_value v && negb (is_error_b v)
     | Constant u    => true
     | Error T       => true
-
-
-    (* Duplication for the termination checker *)
-    | Builtin f   => ltb n (arity f)
-    | Apply nv v  => dec_value' n v && negb (is_error_b v) && dec_value' (S n) nv
-    | TyInst nv T => dec_value' (S n) nv
     | _ => false
   end
   .
 
-Definition dec_value := dec_value' 0.
-
-Definition dec_neutral_value (n : nat) (t : Term) :=
-  match t with
-    | Builtin f   => dec_value' n t
-    | Apply nv v  => dec_value' n t
-    | TyInst nv T => dec_value' n t
-    | _           => false
-  end.
-
 Lemma dec_value_value : forall t, dec_value t = true -> value t.
-Admitted.
-
-Lemma dec_neutral_value_neutral_value : forall n t, dec_neutral_value n t = true -> neutral_value n t.
 Admitted.
